paxos/proof_agreement_chosenProperties.dfy
@@ -1,0 +1,442 @@
+include "types.dfy"
+include "network.dfy"
+include "agents.dfy"
+include "synod.dfy"
+include "proof_helper.dfy"
+include "proof_axioms.dfy"
+include "proof_agreement_invariants.dfy"
+
+module Proof_Agreement_ChosenProperties {
+import opened Network
+import opened Agents
+import opened Types
+import opened Synod
+import opened Proof_Helper
+import opened Proof_Axioms
+import opened Proof_Agreement_Invs
+
+
+// //////////////          Agreement Sub-Lemma: No existing decision          ///////////////
+
+
+lemma AgreementChosenInv_NoneChosen(c:Constants, ds:DistrSys, ds':DistrSys) 
+    requires Agreement_Chosen_Inv(c, ds)
+    requires ds'.WF(c) && Trivialities(c, ds')
+    requires Next(c, ds, ds')
+    requires Agreement_Chosen_Inv_Common(c, ds')
+    requires !SomeValueChosen(c, ds)
+    ensures Agreement_Chosen_Inv_ChosenProperties(c, ds')
+{
+    var actor, recvIos:seq<Packet>, sendIos :| PaxosNextOneAgent(c, ds, ds', actor, recvIos, sendIos);
+    if actor.agt == Ldr {
+        // If actor is a Leader
+        // No values are chosen in this step
+        lemma_NoNewAcceptsImpliesNoNewChosen(c, ds, ds');
+        assert !SomeValueChosen(c, ds');
+    } else {
+        // If actor is an Acceptor: This is the tricky case as 
+        // some value may be chosen in this step
+        AgreementChosenInv_NoneChosen_AccAction(c, ds, ds', actor, recvIos, sendIos);
+    }
+}
+
+
+lemma AgreementChosenInv_NoneChosen_AccAction(
+c:Constants, ds:DistrSys, ds':DistrSys, actor:Id, recvIos:seq<Packet>, sendIos:seq<Packet>)
+    requires Agreement_Chosen_Inv(c, ds)
+    requires ds'.WF(c) && Trivialities(c, ds')
+    requires Agreement_Chosen_Inv_Common(c, ds')
+    requires Next(c, ds, ds')
+    requires PaxosNextOneAgent(c, ds, ds', actor, recvIos, sendIos)
+    requires c.ValidAccId(actor)
+    requires !SomeValueChosen(c, ds)
+    ensures Agreement_Chosen_Inv_ChosenProperties(c, ds')
+{
+    forall b, v | Chosen(c, ds', b, v) 
+    ensures Agreement_Chosen_Inv_SomeValChosen(c, ds', b, v)
+    {
+        lemma_NewChosenImpliesAcceptStep(c, ds, ds', actor, recvIos, sendIos, b, v);
+        AgreementChosenInv_NoneChosen_AccAction_NewChosenV(c, ds, ds', actor, recvIos, sendIos, b, v);
+    }
+}
+
+
+lemma AgreementChosenInv_NoneChosen_AccAction_NewChosenV(
+c:Constants, ds:DistrSys, ds':DistrSys, actor:Id, recvIos:seq<Packet>, sendIos:seq<Packet>, b:Ballot, v:Value)
+    requires Agreement_Chosen_Inv(c, ds)
+    requires ds'.WF(c) && Trivialities(c, ds')
+    requires Agreement_Chosen_Inv_Common(c, ds')
+    requires Next(c, ds, ds')
+    requires PaxosNextOneAgent(c, ds, ds', actor, recvIos, sendIos)
+    requires c.ValidAccId(actor)
+    requires recvIos[0].msg.Propose?
+    requires AcceptorAccept(ds.acceptors[actor.idx], ds'.acceptors[actor.idx], recvIos[0], sendIos);   
+    requires !SomeValueChosen(c, ds)
+    requires Chosen(c, ds', b, v)
+    requires OneValuePerBallot(c, ds');
+    ensures Agreement_Chosen_Inv_SomeValChosen(c, ds', b, v)
+{
+    AgreementChosenInv_NoneChosen_AccAction_NewChosenV_LargerBallotsPromiseQrms(c, ds, ds', actor, recvIos, sendIos, b, v);
+    AgreementChosenInv_NoneChosen_AccAction_NewChosenV_LargerBallotAcceptMsgs(c, ds, ds', actor, recvIos, sendIos, b, v);
+    AgreementChosenInv_NoneChosen_AccAction_NewChosenV_LargerBallotAcceptors(c, ds, ds', actor, recvIos, sendIos, b, v);
+    AgreementChosenInv_NoneChosen_AccAction_NewChosenV_LargerBallotPromiseMsgs(c, ds, ds', actor, recvIos, sendIos, b, v);
+    AgreementChosenInv_NoneChosen_AccAction_NewChosenV_LargerBallotProposeMsgs(c, ds, ds', actor, recvIos, sendIos, b, v);
+    AgreementChosenInv_NoneChosen_AccAction_NewChosenV_P2LeaderV(c, ds, ds', actor, recvIos, sendIos, b, v);
+}
+
+
+lemma AgreementChosenInv_NoneChosen_AccAction_NewChosenV_LargerBallotsPromiseQrms(
+c:Constants, ds:DistrSys, ds':DistrSys, actor:Id, recvIos:seq<Packet>, sendIos:seq<Packet>, b:Ballot, v:Value)
+    requires Agreement_Chosen_Inv(c, ds)
+    requires ds'.WF(c) && Trivialities(c, ds')
+    requires Agreement_Chosen_Inv_Common(c, ds')
+    requires Next(c, ds, ds')
+    requires PaxosNextOneAgent(c, ds, ds', actor, recvIos, sendIos)
+    requires c.ValidAccId(actor)
+    requires recvIos[0].msg.Propose?
+    requires AcceptorAccept(ds.acceptors[actor.idx], ds'.acceptors[actor.idx], recvIos[0], sendIos);   
+    requires !SomeValueChosen(c, ds)
+    requires Chosen(c, ds', b, v)
+    ensures LargerBallotsPromiseQrms(c, ds', b)
+{
+    forall b' | BalLt(b, b') 
+    ensures LargerBalQuorumHasSeenB(c, ds', b, b')
+    {
+        forall qrm':set<Packet> | QuorumOfPromiseMsgs(c, ds', qrm', b') 
+        ensures QuorumHasSeenB(c, ds', qrm', b){
+            AgreementChosenInv_NoneChosen_AccAction_NewChosenV_LargerBallotsPromiseQrms_helper(c, ds, ds', actor, recvIos, sendIos, b, b', qrm', v);
+        }
+    }
+}
+
+lemma AgreementChosenInv_NoneChosen_AccAction_NewChosenV_LargerBallotsPromiseQrms_helper(
+c:Constants, ds:DistrSys, ds':DistrSys, actor:Id, recvIos:seq<Packet>, sendIos:seq<Packet>, b:Ballot, b':Ballot, qrm':set<Packet>, v:Value)
+    requires Agreement_Chosen_Inv(c, ds)
+    requires ds'.WF(c) && Trivialities(c, ds')
+    // Picking individual items from Agreement_Chosen_Inv_Common, faster verification
+    requires OneValuePerBallot(c, ds')
+    requires PromiseMsgImpliesPromised(c, ds')
+    requires PromisedImpliesNoMoreAccepts(c, ds')
+    requires AccPromisedBallotLargerThanAccepted(c, ds')
+    requires AcceptMsgImpliesAccepted(c, ds')
+
+    requires Next(c, ds, ds')
+    requires PaxosNextOneAgent(c, ds, ds', actor, recvIos, sendIos)
+    requires c.ValidAccId(actor)
+    requires recvIos[0].msg.Propose?
+    requires AcceptorAccept(ds.acceptors[actor.idx], ds'.acceptors[actor.idx], recvIos[0], sendIos)   
+    requires !SomeValueChosen(c, ds)
+    requires Chosen(c, ds', b, v)
+    requires BalLt(b, b') 
+    requires QuorumOfPromiseMsgs(c, ds', qrm', b')
+    ensures QuorumHasSeenB(c, ds', qrm', b)
+{
+    /* Proof: Suppose otherwise. Then qrm' is in ds, and every Prom in qrm' has promised
+    * b', and saw < b. By PromisedImpliesNoMoreAccepts, this means that no Accept(b) messages
+    * from any acceptor in qrm'.
+    * Call the set of acceptors that chose (b, v) in ds' as qrm. Then qrm and qrm' must be disjoint, 
+    * and their union is the set of all acceptors, and qrm is size f. 
+    * Now consider the actor taking a step: 
+    *   1. If actor is in qrm', it can't accept (b, v). Hence (b,v) not chosen in ds'. C!
+    *   2. If actor is in qrm, |qrm| remains f in ds'. C!
+    */
+    if !QuorumHasSeenB(c, ds', qrm', b) {
+        forall prom | prom in qrm' ensures BalLt(prom.msg.vb.b, b) {}
+        lemma_NoPromiseSentInNonPromiseStep(c, ds, ds', actor, recvIos, sendIos);
+        assert QuorumOfPromiseMsgs(c, ds, qrm', b');
+        
+        // Get set of acceptors that promised b' (and not seen b) in ds
+        var accs_that_promised := extractPacketSources(qrm');
+        assert |accs_that_promised| >= c.f + 1;
+
+        // Get set of acceptors that voted to choose (b, v) in ds
+        var qrm :| QuorumOfAcceptMsgs(c, ds', qrm, b) && AccPacketsHaveValueV(qrm, v);
+        var new_accept_pkt := lemma_NewChosenImpliesOneNewAcceptPacket(c, ds, ds', actor, recvIos, sendIos, b, v);
+        var pre_qrm := qrm - {new_accept_pkt};   // set without the latest Accept from ds->ds' actor.
+        assert SetOfAcceptMsgs(c, ds, pre_qrm, b);
+        lemma_Set_MinusElem(qrm, new_accept_pkt, |qrm|);
+        var accs_that_accepted := extractPacketSources(pre_qrm);
+        assert |accs_that_accepted| >= c.f;
+
+        // Show that accs_that_promised && accs_that_accepted are disjoint;
+        // use PromisedImpliesNoMoreAccepts
+        forall id | id in accs_that_promised 
+        ensures id !in accs_that_accepted
+        {
+            var prom :| prom in qrm' && prom.src == id;
+            forall accp | accp in qrm 
+            ensures accp.src != id
+            {
+                if accp.src == id {      
+                    assert !BalLtEq(accp.msg.bal, prom.msg.vb.b);
+                    lemma_BalLtSynonyms(b, b');
+                    assert !BalLtEq(prom.msg.bal, accp.msg.bal);
+                    assert false;
+                }
+            }
+        }
+        axiom_Set_DisjointSets(accs_that_promised, accs_that_accepted);
+        // Consider the current actor taking a step
+        lemma_IdSetCover(c, ds, accs_that_promised, accs_that_accepted, actor);
+        if actor in accs_that_promised {
+            assert BalLtEq(b', ds.acceptors[actor.idx].promised);   // by PromiseMsgImpliesPromised
+            lemma_BalLtTransitivity1(b, b', ds.acceptors[actor.idx].promised);
+            lemma_NewChosenImpliesIncomingProposalBV(c, ds, ds', actor, recvIos, sendIos, b, v);
+            assert !AcceptorAccept(ds.acceptors[actor.idx], ds'.acceptors[actor.idx], recvIos[0], sendIos); 
+            assert false;
+        } else {
+            assert actor in accs_that_accepted;
+            var p :| p in pre_qrm && p.src == actor && isAcceptPkt(ds, p) && p.msg.bal == b;
+            lemma_NewChosenImpliesIncomingProposalBV(c, ds, ds', actor, recvIos, sendIos, b, v);
+            assert sendIos[0] == p;
+            assert ds'.network.sentPackets == ds.network.sentPackets;
+            assert false;       // violates lemma_NewChosenImpliesOneNewAcceptPacket
+        }
+    }
+}
+
+
+lemma AgreementChosenInv_NoneChosen_AccAction_NewChosenV_LargerBallotAcceptMsgs(
+c:Constants, ds:DistrSys, ds':DistrSys, actor:Id, recvIos:seq<Packet>, sendIos:seq<Packet>, b:Ballot, v:Value)
+    requires Agreement_Chosen_Inv(c, ds)
+    requires ds'.WF(c) && Trivialities(c, ds')
+    requires Agreement_Chosen_Inv_Common(c, ds')
+    requires Next(c, ds, ds')
+    requires PaxosNextOneAgent(c, ds, ds', actor, recvIos, sendIos)
+    requires c.ValidAccId(actor)
+    requires recvIos[0].msg.Propose?
+    requires AcceptorAccept(ds.acceptors[actor.idx], ds'.acceptors[actor.idx], recvIos[0], sendIos)   
+    requires !SomeValueChosen(c, ds)
+    requires Chosen(c, ds', b, v)
+    requires LargerBallotsPromiseQrms(c, ds', b)
+    ensures LargerBallotAcceptMsgs(c, ds', b, v)
+{
+    forall accpt | isAcceptPkt(ds', accpt) && BalLtEq(b, accpt.msg.bal)
+    ensures accpt.msg.val == v
+    {
+        AgreementChosenInv_NoneChosen_AccAction_NewChosenV_LargerBallotAcceptMsgs_helper(c, ds, ds', 
+            actor, recvIos, sendIos, b, v, accpt, accpt.msg.bal, accpt.msg.val);
+    }
+}
+
+
+lemma AgreementChosenInv_NoneChosen_AccAction_NewChosenV_LargerBallotAcceptMsgs_helper(
+c:Constants, ds:DistrSys, ds':DistrSys, actor:Id, recvIos:seq<Packet>, sendIos:seq<Packet>, b:Ballot, v:Value,
+accpt:Packet, b1:Ballot, v':Value)
+    decreases b1
+    requires Agreement_Chosen_Inv(c, ds)
+    requires ds'.WF(c) && Trivialities(c, ds')
+    // Picking individual items from Agreement_Chosen_Inv_Common, faster verification
+    // requires Agreement_Chosen_Safety(c, ds') 
+    requires OneValuePerBallot(c, ds')
+    requires AcceptMsgImpliesProposeMsg(c, ds')
+    requires ProposeMsgImpliesQuorumOfPromise(c, ds')
+    requires PromiseVBImpliesAcceptMsg(c, ds')
+    requires PromiseMsgBalLargerThanAcceptedItSees(c, ds')
+
+    requires Next(c, ds, ds')
+    requires PaxosNextOneAgent(c, ds, ds', actor, recvIos, sendIos)
+    requires c.ValidAccId(actor)
+    requires recvIos[0].msg.Propose?
+    requires AcceptorAccept(ds.acceptors[actor.idx], ds'.acceptors[actor.idx], recvIos[0], sendIos)
+    requires !SomeValueChosen(c, ds)
+    requires Chosen(c, ds', b, v)
+    requires LargerBallotsPromiseQrms(c, ds', b)
+    requires isAcceptPkt(ds', accpt) && BalLtEq(b, accpt.msg.bal)
+    requires b1 == accpt.msg.bal
+    requires v' == accpt.msg.val
+    ensures accpt.msg.val == v
+{
+    /* Consider accpt Accept(b1, v') message, b1 >b. By AcceptMsgImpliesProposeMsg, there is a Propose(b1, v') in the network.
+    * By ProposeMsgImpliesQuorumOfPromise, there is a quorum qrm1 of promise b1 packets, such that 
+    * PromisePktWithHighestBallot(qrm1).msg.vb.v == v'. By LargerBallotsPromiseQrms, qrm1 must also see (b, v).
+    * There are now two cases:
+    *   1. PromisePktWithHighestBallot(qrm1).msg.vb.b == b. Then we are done, by OneValuePerBallot.
+    *   2. PromisePktWithHighestBallot(qrm1).msg.vb.b == b2. By PromiseMsgBalLargerThanAcceptedItSees, b2 < b1.
+    *          I.e. b < b2 < b1.
+    * This means that there is a Accept(b2, v') message. And we go down recursively. 
+    * Since there are finite number of ballots (say, i) between b1 and b, after i iterations of step 2, 
+    * we must hit b eventually, and QED.
+    */
+    var b1, v' := accpt.msg.bal, accpt.msg.val;
+    if b1 == b {
+        var chosen_qrm_member :|    && isAcceptPkt(ds', chosen_qrm_member)
+                                    && chosen_qrm_member.msg.bal == b
+                                    && chosen_qrm_member.msg.val == v;
+        assert chosen_qrm_member.msg.val == accpt.msg.val;  // by OneValuePerBallot_AcceptMsg
+    } else {
+        var prop1 :| isProposePkt(ds', prop1) && prop1.msg == Propose(b1, v');
+        var qrm1 :| QuorumOfPromiseMsgs(c, ds', qrm1, b1)
+                    && (|| PromisePktWithHighestBallot(qrm1).msg.vb.v == v'
+                        || PromisePktWithHighestBallot(qrm1).msg.vb.v == Nil);
+        var prom1 := PromisePktWithHighestBallot(qrm1);
+        // The highest ballot in qrm1 is not Nil
+        if prom1.msg.vb.v == Nil {
+            lemma_HighestPromiseValNilImpliesAllBottom(qrm1);
+            assert !QuorumHasSeenB(c, ds', qrm1, b);
+            assert false;
+        }
+        assert isPromisePkt(ds', prom1) && prom1.msg.vb.b != Bottom;
+
+        // Establish b <= b2 < b1
+        var b2 := prom1.msg.vb.b;
+        var b_witness:Packet :| b_witness in qrm1 && BalLtEq(b, b_witness.msg.vb.b);    // by LargerBallotsPromiseQrms
+        lemma_BalLtEqTransitivity(b, b_witness.msg.vb.b, b2);
+        assert BalLtEq(b, b2);
+        assert BalLt(b2, b1);       // by PromiseMsgBalLargerThanAcceptedItSees
+
+        // Fetch Accept packet corresponding to balval seen by prom1
+        var accpt2 :|   && isAcceptPkt(ds', accpt2)      // by PromiseVBImpliesAcceptMsg
+                        && accpt2.msg == Accept(b2, v');
+        // AgreementChosenInv_NoneChosen_AccAction_NewChosenV_LargerBallotAcceptMsgs_helper(c, ds, ds', 
+        //     actor, recvIos, sendIos, b, v, accpt2, b2, v');
+        axiom_BallotInduction1(c, ds', accpt, b, v);
+    }
+}
+
+
+lemma AgreementChosenInv_NoneChosen_AccAction_NewChosenV_LargerBallotAcceptors(
+c:Constants, ds:DistrSys, ds':DistrSys, actor:Id, recvIos:seq<Packet>, sendIos:seq<Packet>, b:Ballot, v:Value)
+    requires Agreement_Chosen_Inv(c, ds)
+    requires ds'.WF(c) && Trivialities(c, ds')
+    requires Agreement_Chosen_Inv_Common(c, ds')
+    requires Next(c, ds, ds')
+    requires PaxosNextOneAgent(c, ds, ds', actor, recvIos, sendIos)
+    requires c.ValidAccId(actor)
+    requires recvIos[0].msg.Propose?
+    requires AcceptorAccept(ds.acceptors[actor.idx], ds'.acceptors[actor.idx], recvIos[0], sendIos);   
+    requires !SomeValueChosen(c, ds)
+    requires Chosen(c, ds', b, v)
+    requires LargerBallotsPromiseQrms(c, ds', b)
+    requires LargerBallotAcceptMsgs(c, ds', b, v)
+    ensures LargerBallotAcceptors(c, ds', b, v)
+{
+    forall i' | c.ValidAccIdx(i') && BalLtEq(b, ds'.acceptors[i'].accepted.b)
+    ensures AcceptorHasValueV(c, ds', i', v) {
+        var b', v' :=  ds'.acceptors[i'].accepted.b, ds'.acceptors[i'].accepted.v;
+        if v' != v {
+            var accp :| && isAcceptPkt(ds', accp)   // by AcceptedImpliesAcceptMsg
+                        && accp.msg == Accept(b', v');
+            assert false;   // violtes LargerBallotAcceptMsgs
+        }
+    }
+}
+
+
+
+lemma AgreementChosenInv_NoneChosen_AccAction_NewChosenV_LargerBallotPromiseMsgs(
+c:Constants, ds:DistrSys, ds':DistrSys, actor:Id, recvIos:seq<Packet>, sendIos:seq<Packet>, b:Ballot, v:Value)
+    requires Agreement_Chosen_Inv(c, ds)
+    requires ds'.WF(c) && Trivialities(c, ds')
+    requires Agreement_Chosen_Inv_Common(c, ds')
+    requires Next(c, ds, ds')
+    requires PaxosNextOneAgent(c, ds, ds', actor, recvIos, sendIos)
+    requires c.ValidAccId(actor)
+    requires !SomeValueChosen(c, ds)
+    requires Chosen(c, ds', b, v)
+    requires LargerBallotAcceptMsgs(c, ds', b, v)
+    ensures LargerBallotPromiseMsgs(c, ds', b, v)
+{
+    forall p | isPromisePkt(ds', p) && BalLtEq(b, p.msg.vb.b)
+    ensures p.msg.vb.v == v 
+    {
+        var b', v' := p.msg.vb.b, p.msg.vb.v;
+        var ap :|  && isAcceptPkt(ds', ap)
+                    && ap.src == p.src
+                    && ap.msg.bal == b'
+                    && ap.msg.val == v';
+        assert LargerBallotAcceptMsgs(c, ds', b, v);
+        if v' != v {
+            assert false;
+        }
+    }
+}
+
+
+lemma AgreementChosenInv_NoneChosen_AccAction_NewChosenV_LargerBallotProposeMsgs(
+c:Constants, ds:DistrSys, ds':DistrSys, actor:Id, recvIos:seq<Packet>, sendIos:seq<Packet>, b:Ballot, v:Value)
+    requires Agreement_Chosen_Inv(c, ds)
+    requires ds'.WF(c) && Trivialities(c, ds')
+    requires Agreement_Chosen_Inv_Common(c, ds')
+    requires Next(c, ds, ds')
+    requires PaxosNextOneAgent(c, ds, ds', actor, recvIos, sendIos)
+    requires c.ValidAccId(actor)
+    requires !SomeValueChosen(c, ds)
+    requires Chosen(c, ds', b, v)
+    requires LargerBallotPromiseMsgs(c, ds', b, v)
+    requires LargerBallotsPromiseQrms(c, ds', b)
+    ensures LargerBallotProposeMsgs(c, ds', b, v)
+{
+    forall p | isProposePkt(ds', p) && BalLtEq(b, p.msg.bal)
+    ensures p.msg.val == v
+    {
+        var b', v' := p.msg.bal, p.msg.val;
+        if b' == b {
+            assert v == v';     // by OneValuePerBallot_ProposeMsg
+        } else {
+            var prom_qrm :| && QuorumOfPromiseMsgs(c, ds', prom_qrm, b')
+                            && (|| PromisePktWithHighestBallot(prom_qrm).msg.vb.v == v'
+                                || PromisePktWithHighestBallot(prom_qrm).msg.vb.v == Nil);
+            var prom := PromisePktWithHighestBallot(prom_qrm);
+            var prom_smaller:Packet :| prom_smaller in prom_qrm && BalLtEq(b, prom_smaller.msg.vb.b);  // because Quorum must have seen b (LargerBallotsPromiseQrms)
+            lemma_BalLtEqTransitivity(b, prom_smaller.msg.vb.b, prom.msg.vb.b);
+            assert PromisePktWithHighestBallot(prom_qrm).msg.vb.v == v;     // because LargerBallotPromiseMsgs
+        }
+    }
+}
+
+
+lemma AgreementChosenInv_NoneChosen_AccAction_NewChosenV_P2LeaderV(
+c:Constants, ds:DistrSys, ds':DistrSys, actor:Id, recvIos:seq<Packet>, sendIos:seq<Packet>, b:Ballot, v:Value)
+    requires Agreement_Chosen_Inv(c, ds)
+    requires ds'.WF(c) && Trivialities(c, ds')
+    requires Agreement_Chosen_Inv_Common(c, ds')
+    requires Next(c, ds, ds')
+    requires PaxosNextOneAgent(c, ds, ds', actor, recvIos, sendIos)
+    requires c.ValidAccId(actor)
+    requires recvIos[0].msg.Propose?
+    requires AcceptorAccept(ds.acceptors[actor.idx], ds'.acceptors[actor.idx], recvIos[0], sendIos);   
+    requires !SomeValueChosen(c, ds)
+    requires Chosen(c, ds', b, v)
+    requires LargerBallotsPromiseQrms(c, ds', b)
+    requires LargerBallotPromiseMsgs(c, ds', b, v)
+    ensures LargerBallotPhase2LeadersV(c, ds', b, v)
+{
+    forall l_idx |  && c.ValidLdrIdx(l_idx) 
+                    && BalLtEq(b, ds'.leaders[l_idx].ballot) 
+                    && LeaderInPhase2(c, ds', l_idx) 
+    ensures LeaderHasValueV(c, ds', l_idx, v)
+    {
+        if !LeaderHasValueV(c, ds', l_idx, v) {
+            var b', v' := ds'.leaders[l_idx].ballot, ds'.leaders[l_idx].val;
+            assert v' != v;
+            if b' == b {
+                var prop_p := lemma_ChosenImpliesProposeMsg(c, ds', b, v);
+                assert v == v';
+                assert false; 
+            } else {
+                assert BalLt(b, b');
+                var qrm' :| && QuorumOfPromiseMsgs(c, ds', qrm', b')
+                            && (|| PromisePktWithHighestBallot(qrm').msg.vb.v == v'
+                                || PromisePktWithHighestBallot(qrm').msg.vb.v == Nil);
+                if PromisePktWithHighestBallot(qrm').msg.vb.v == Nil {
+                    lemma_HighestPromiseValNilImpliesAllBottom(qrm');
+                    assert !QuorumHasSeenB(c, ds', qrm', b);
+                    assert false;
+                } else {
+                    var pivot:Packet :| pivot in qrm' && BalLtEq(b, pivot.msg.vb.b);
+                    assert pivot.msg.vb.v == v;
+                    forall p:Packet | p in qrm' && BalLtEq(pivot.msg.vb.b, p.msg.vb.b) 
+                    ensures p.msg.vb.v == v {
+                        lemma_BalLtEqTransitivity(b, pivot.msg.vb.b, p.msg.vb.b);
+                    }
+                    lemma_PromisePktWithHighestBallotProperty(qrm', pivot, v);
+                    assert PromisePktWithHighestBallot(qrm').msg.vb.v == v;
+                    assert false;
+                }
+            }
+        }
+    }
+}
+
+}
